\chapter{\texorpdfstring{Legame tra \(\hat{L}^2\) e \(\hat{p}^2\)}{}}

\begin{gather*}
    \hat{L}^2 = (\vec{x}\times \vec{p}) = \sum_{ijkls = 1}^3 \varepsilon_{ijk} \hat{x}_j \hat{p}_k \varepsilon^{ils}\hat{x}^l\hat{p}^s \\
    \varepsilon_{ijk} \varepsilon^{ils} = \delta^l_j \delta^s_k - \delta^i_j \delta^l_k \tag{a}\\
    \hat{L}^2 = \hat{x}_j\hat{p}_k \hat{x}_j \hat{p}_k - \hat{x}_j \hat{p}_k \hat{x}_k \hat{p}_j = \hat{x}_j (\hat{x}_j \hat{p}_k - i\hslash \delta_{jk}) \hat{p}_k - \hat{x}_j \hat{p}_k (\hat{p}_j \hat{x}_k + i \hslash \delta_{jk}) \\
    \hat{L}^2 = \hat{x}^2 \hat{p}^2 - {(\hat{\vec{x}}\cdot \hat{\vec{x}})}^2 + i\hslash(\hat{\vec{x}}\cdot \hat{\vec{x}}) \tag{0}
\end{gather*}

